LeanMove/Examples/initial/accepted/deref_borrow_field_ok.lean
@@ -19,7 +19,7 @@ import Ssreflect.Lang
 
 import LeanMove.Lang.MoveLight
 import LeanMove.Checker.TypeChecking
-import LeanMove.Checker.TypeCheckingAlgorithmic
+import LeanMove.Checker.Algorithmic.TypeCheckingAlgorithmic
 import LeanMove.Lang.Macros
 
 -- -----------------------------------------------------
